Veritas.Verifier.fst
@@ -16,29 +16,25 @@ open Veritas.MultiSetHash
  *)
 
 (* Each entry of the verifier log *)
-type vlog_entry =
-  | Get: k:data_key -> v:data_value -> vlog_entry
-  | Put: k:data_key -> v:data_value -> vlog_entry
-  | AddM: r:record -> k':merkle_key -> vlog_entry
-  | EvictM: k:key -> k':merkle_key -> vlog_entry
-  | AddB: r:record -> t:timestamp -> j:nat -> vlog_entry
-  | EvictB: k:key -> t:timestamp -> vlog_entry
-  | EvictBM: k:key -> k':merkle_key -> t:timestamp -> vlog_entry
-
-(* verifier log entry (global)  *)
-type vlog_entry_g (#p:pos) =
-  | TOp: tid:nat{tid < p} -> e:vlog_entry -> vlog_entry_g #p
+type vlog_entry (#p:nat) =
+  | Get: k:data_key -> v:data_value -> vlog_entry #p
+  | Put: k:data_key -> v:data_value -> vlog_entry #p
+  | AddM: r:record -> k':merkle_key -> vlog_entry #p
+  | EvictM: k:key -> k':merkle_key -> vlog_entry #p
+  | AddB: r:record -> t:timestamp -> j:nat -> vlog_entry #p
+  | EvictB: k:key -> t:timestamp -> vlog_entry #p
+  | EvictBM: k:key -> k':merkle_key -> t:timestamp -> vlog_entry #p
 
 (* verifier log *)
-type vlog (#p:pos) = seq (vlog_entry_g #p)
+type vlog (#p:nat) = seq (vlog_entry #p)
 
 (* index in the verifier log *)
 type vl_index (#p:pos) (l:vlog #p) = seq_index l
 
 (* for records in the store, how were they added? *)
 type add_method =
-  | Merkle: add_method       (* AddM *)
-  | Blum: add_method         (* AddB *)
+  | MAdd: add_method       (* AddM *)
+  | BAdd: add_method         (* AddB *)
 
 (* verifier store entry *)
 type vstore_entry (k:key) =
@@ -48,24 +44,19 @@ type vstore_entry (k:key) =
 (* we also track how the key was added merkle/blum *)
 type vstore = (k:key) -> option (vstore_entry k)
 
-(* verifier thread local state  *)
-noeq type vtls =
-  | TLS: st:vstore -> clk:timestamp -> lk:key -> vtls
-
 (* per-epoch hash value *)
 type epoch_hash = nat -> ms_hash_value
 
-(* verifier global state *)
-noeq type vgs =
-  | GS: hadd: epoch_hash ->
-        hevict: epoch_hash -> vgs
-
-(* verifier state aggregated across all verifier threads *)
-noeq type vstate (p:pos) =
-  | Failed: vstate p
-  | Valid: tlss:seq vtls{length tlss = p} ->
-           gs:vgs ->
-           vstate p
+(* verifier thread local state  *)
+noeq type vtls (#p:pos) =
+  | Failed
+  | Valid: id:nat{id < p} ->
+           st:vstore -> 
+           clk:timestamp -> 
+           lk:key -> 
+           hadd: epoch_hash ->
+           hevict: epoch_hash ->
+           vtls #p
 
 (* does the store contain address a *)
 let store_contains (st:vstore) (k:key) = Some? (st k)
@@ -100,72 +91,51 @@ let evict_from_store (st:vstore)
                      (k:key{store_contains st k}) =
   fun k' -> if k' = k then None else st k'
 
+let thread_id (#p:pos) (vs:vtls #p {Valid? vs}): i:nat{i < p} = 
+  Valid?.id vs
+
 (* get the store of a specified verifier thread *)
-let thread_store (#p:pos) (i:nat{i < p}) (vs:vstate p{Valid? vs}): vstore =
-  let tlss = Valid?.tlss vs in
-  let tls = index tlss i in
-  TLS?.st tls
+let thread_store (#p:pos) (vs: vtls #p {Valid? vs}): vstore =
+  Valid?.st vs
 
 (* update the store of a specified verifier thread *)
-let update_thread_store (#p:pos)
-                        (i:nat{i < p})
-                        (vs:vstate p{Valid? vs})
+let update_thread_store (#p:pos) 
+                        (vs:vtls #p{Valid? vs})
                         (st:vstore)
-                        : vstate p =
-  let tlss = Valid?.tlss vs in
-  let gs = Valid?.gs vs in
-  let tls = index tlss i in
-  match tls with
-  | TLS _ clk lk -> let tls' = TLS st clk lk in
-                    let tlss' = upd tlss i tls' in
-                    Valid tlss' gs
+                        : vtls #p =
+  match vs with
+  | Valid id _ clk lk ha he -> Valid id st clk lk ha he
 
-let thread_clock (#p:pos) (i:nat{i < p}) (vs:vstate p{Valid? vs}) = 
-  let tlss = Valid?.tlss vs in
-  let tls = index tlss i in
-  TLS?.clk tls
+(* get the clock from verifier thread state *)
+let thread_clock (#p:pos) (vs:vtls #p{Valid? vs}) = 
+  Valid?.clk vs
 
+(* update the clock of the verifier *)
+let update_thread_clock (#p:pos) (vs:vtls #p {Valid? vs})
+                        (clk:timestamp): vtls #p = 
+  match vs with
+  | Valid id st _ lk ha he -> Valid id st clk lk ha he
 
-let update_thread_clock (#p:pos) (i:nat{i < p})
-                        (vs:vstate p{Valid? vs})
-                        (clk:timestamp): vstate p = 
-  let tlss = Valid?.tlss vs in
-  let gs = Valid?.gs vs in
-  let tls = index tlss i in
-  match tls with
-  | TLS st _ lk -> let tls' = TLS st clk lk in
-                   let tlss' = upd tlss i tls' in
-                   Valid tlss' gs
+let thread_hadd (#p:pos) (vs:vtls #p{Valid? vs}) = 
+  Valid?.hadd vs
 
-let hadd (#p:pos) (e:nat) (vs:vstate p{Valid? vs}) = 
-  let gs = Valid?.gs vs in
-  let h = GS?.hadd gs in
-  h e
-
-let hevict (#p:pos) (e:nat) (vs:vstate p{Valid? vs}) = 
-  let gs = Valid?.gs vs in
-  let h = GS?.hevict gs in
-  h e
+let thread_hevict (#p:pos) (vs:vtls #p{Valid? vs}) = 
+  Valid?.hevict vs
 
 let update_epoch_hash (eh: epoch_hash) (e:nat) (h:ms_hash_value) = 
   fun e' -> if e = e' then h else eh e'
 
-let update_hadd (#p:pos) (e:nat) (h: ms_hash_value)  (vs:vstate p{Valid? vs}): vstate p = 
+let update_thread_hadd (#p:pos) (vs:vtls #p {Valid? vs}) (e:nat) (h: ms_hash_value): vtls #p = 
   match vs with
-  | Valid tlss gs -> match gs with
-                    | GS ha he -> let gs' = GS (update_epoch_hash ha e h) he in
-                                  Valid tlss gs'
+  | Valid id st clk lk ha he -> Valid id st clk lk (update_epoch_hash ha e h) he
 
-let update_hevict (#p:pos) (e:nat) (h:ms_hash_value) (vs:vstate p{Valid? vs}): vstate p = 
+let update_thread_hevict (#p:pos) (vs:vtls #p {Valid? vs}) (e:nat) (h:ms_hash_value): vtls #p = 
   match vs with
-  | Valid tlss gs -> match gs with
-                    | GS ha he -> let gs' = GS ha (update_epoch_hash he e h) in
-                                  Valid tlss gs'
+  | Valid id st clk lk ha he -> Valid id st clk lk ha (update_epoch_hash he e h)
 
 (* verifier read operation *)
-let vget (#p:pos) (i:nat{i < p})
-         (k:data_key) (v:data_value) (vs: vstate p{Valid? vs}): vstate p =
-  let st = thread_store i vs in
+let vget (#p:pos) (k:data_key) (v:data_value) (vs: vtls #p{Valid? vs}): vtls #p =
+  let st = thread_store vs in
   (* check store contains key *)
   if not (store_contains st k) then Failed
   (* check stored value is v *)
@@ -174,12 +144,11 @@ let vget (#p:pos) (i:nat{i < p})
   else vs
   
 (* verifier write operation *)
-let vput (#p:pos) (i:nat{i < p})
-         (k:data_key) (v:data_value) (vs: vstate p{Valid? vs}): vstate p =
-  let st = thread_store i vs in
+let vput (#p:pos) (k:data_key) (v:data_value) (vs: vtls #p{Valid? vs}): vtls #p =
+  let st = thread_store vs in
   (* check store contains key *)
   if not (store_contains st k) then Failed
-  else update_thread_store i vs (update_store st k (DVal v))
+  else update_thread_store vs (update_store st k (DVal v))
 
 (* update merkle value *)
 let update_merkle_value (v:merkle_value)
@@ -192,11 +161,11 @@ let update_merkle_value (v:merkle_value)
                       | Left -> MkValue (Desc k h b) dhr
                       | Right -> MkValue dhl (Desc k h b)
 
-let vaddm (#p:pos) (i:nat{i < p})
+let vaddm (#p:pos)
           (r:record)
           (k':merkle_key)
-          (vs: vstate p{Valid? vs}): vstate p =
-  let st = thread_store i vs in
+          (vs: vtls #p{Valid? vs}): vtls #p =
+  let st = thread_store vs in
   let (k,v) = r in
   (* check k is a proper desc of k' *)
   if not (is_proper_desc k k') then Failed
@@ -215,12 +184,12 @@ let vaddm (#p:pos) (i:nat{i < p})
     | Empty -> if v = init_value k then
                  let v'_upd = update_merkle_value v' d k h false in
                  let st_upd = update_store st k' (MVal v'_upd) in
-                 let st_upd2 = add_to_store st_upd k v Merkle in
-                 update_thread_store i vs st_upd2
+                 let st_upd2 = add_to_store st_upd k v MAdd in
+                 update_thread_store vs st_upd2
                else Failed
     | Desc k2 h2 b2 -> if k2 = k then
                          if h2 = h then
-                           update_thread_store i vs (add_to_store st k v Merkle)
+                           update_thread_store vs (add_to_store st k v MAdd)
                          else Failed
                        else if v <> init_value k then Failed
                        else if not (is_proper_desc k2 k) then Failed
@@ -230,14 +199,14 @@ let vaddm (#p:pos) (i:nat{i < p})
                          let mv_upd = update_merkle_value mv d2 k2 h2 b2 in
                          let v'_upd = update_merkle_value v' d k h false in
                          let st_upd = update_store st k'(MVal  v'_upd) in
-                         let st_upd2 = add_to_store st_upd k (MVal mv_upd) Merkle in
-                         update_thread_store i vs st_upd2
+                         let st_upd2 = add_to_store st_upd k (MVal mv_upd) MAdd in
+                         update_thread_store vs st_upd2
 
-let vevictm (#p:pos) (i:nat{i < p})
+let vevictm (#p:pos) 
             (k:key)
             (k':merkle_key)
-            (vs: vstate p{Valid? vs}): vstate p = 
-  let st = thread_store i vs in
+            (vs: vtls #p{Valid? vs}): vtls #p = 
+  let st = thread_store vs in
   (* check store contains a and a' *)
   if not (store_contains st k && store_contains st k') then Failed
   else if not (is_proper_desc k k') then Failed
@@ -252,22 +221,20 @@ let vevictm (#p:pos) (i:nat{i < p})
     | Desc k2 h2 b2 -> if k2 = k then
                          let v'_upd = update_merkle_value v' d k h b2 in
                          let st_upd = evict_from_store (update_store st k' (MVal v'_upd)) k in
-                         update_thread_store i vs st_upd
+                         update_thread_store vs st_upd
                        else Failed
 
 let max (t1 t2: timestamp) = 
   if t1 `ts_lt` t2 then t2 else t1
 
-let vaddb (#p:pos) (i:nat{i < p})
+let vaddb (#p:pos)
           (r:record)
           (t:timestamp)
           (j:nat)
-          (vs:vstate p{Valid? vs}): vstate p = 
-  (* global state *)
-  let gs = Valid?.gs vs in          
+          (vs:vtls #p{Valid? vs}): vtls #p = 
   (* epoch of timestamp of last evict *)
   let e = MkTimestamp?.e t in
-  let st = thread_store i vs in  
+  let st = thread_store vs in  
   let (k,v) = r in
   (* check value type consistent with key k *)
   if not (is_value_of k v) then Failed
@@ -275,44 +242,41 @@ let vaddb (#p:pos) (i:nat{i < p})
   else if store_contains st k then Failed
   else 
     (* current h_add *)
-    let h = hadd e vs in
+    let h = thread_hadd vs e in
     (* updated h_add *)
     let h_upd = ms_hashfn_upd (MHDom r t j) h in
     (* update verifier state *)
-    let vs_upd = update_hadd e h_upd vs in
+    let vs_upd = update_thread_hadd vs e h_upd in
     (* current clock of thread i *)
-    let clk = thread_clock i vs in
+    let clk = thread_clock vs in
     (* updated clock *)
     let clk_upd = max clk t in
     (* update verifier state with new clock *)
-    let vs_upd2 = update_thread_clock i vs_upd clk_upd in
+    let vs_upd2 = update_thread_clock vs_upd clk_upd in
     (* add record to store *)
-    let st_upd = add_to_store st k v Blum in
-    update_thread_store i vs_upd2 st_upd
+    let st_upd = add_to_store st k v BAdd in
+    update_thread_store vs_upd2 st_upd
 
-let vevictb (#p:pos) (i:nat{i < p})
-            (k:key) (t:timestamp)
-            (vs:vstate p{Valid? vs}): vstate p = 
-  let gs = Valid?.gs vs in
-  let clk = thread_clock i vs in
+let vevictb (#p:pos) (k:key) (t:timestamp)
+            (vs:vtls #p{Valid? vs}): vtls #p = 
+  let clk = thread_clock vs in
   let e = MkTimestamp?.e t in
-  let st = thread_store i vs in
+  let st = thread_store vs in
   if not (ts_lt clk t) then Failed
   else if not (store_contains st k) then Failed  
   else 
     (* current h_evict *)
-    let h = hevict e vs in
+    let h = thread_hevict vs e in
     let v = stored_value st k in
-    let h_upd = ms_hashfn_upd (MHDom (k,v) t i) h in
-    let vs_upd = update_hevict e h_upd vs in
-    let vs_upd2 = update_thread_clock i vs_upd t in    
+    let h_upd = ms_hashfn_upd (MHDom (k,v) t (thread_id vs)) h in
+    let vs_upd = update_thread_hevict vs e h_upd in
+    let vs_upd2 = update_thread_clock vs_upd t in    
     let st_upd = evict_from_store st k in
-    update_thread_store i vs_upd2 st_upd
+    update_thread_store vs_upd2 st_upd
 
-let vevictbm (#p:pos) (i:nat{i < p})
-             (k:key) (k':merkle_key) (t:timestamp)
-             (vs:vstate p{Valid? vs}): vstate p = 
-  let st = thread_store i vs in
+let vevictbm (#p:pos) (k:key) (k':merkle_key) (t:timestamp)
+             (vs:vtls #p{Valid? vs}): vtls #p = 
+  let st = thread_store vs in
   if not (store_contains st k') then Failed 
   else if not (is_proper_desc k k') then Failed
   else
@@ -324,54 +288,48 @@ let vevictbm (#p:pos) (i:nat{i < p})
     | Desc k2 h2 b2 -> if k2 = k && b2 = false then
                          let v'_upd = update_merkle_value v' d k h2 true in
                          let st_upd = update_store st k' (MVal v'_upd) in
-                         vevictb i k t (update_thread_store i vs st_upd)
+                         vevictb k t (update_thread_store vs st_upd)
                        else Failed
  
-let verifier_step_thread (#p:pos)
-                         (e:vlog_entry)
-                         (i:nat{i < p})
-                         (vs:vstate p{Valid? vs}): vstate p =                           
-  match e with
-  | Get k v -> vget i k v vs
-  | Put k v -> vput i k v vs
-  | AddM r k'  -> vaddm i r k' vs
-  | EvictM k k' -> vevictm i k k' vs
-  | AddB r t j -> vaddb i r t j vs
-  | EvictB k t -> vevictb i k t vs
-  | EvictBM k k' t -> vevictbm i k k' t vs
-
-let verifier_step (#p:pos) (e:vlog_entry_g #p) (vs:vstate p): vstate p =
+let verifier_thread_step (#p:pos)
+                         (e:vlog_entry #p)
+                         (vs:vtls #p): vtls #p =                           
   match vs with
-  | Failed -> Failed              // propagate failures
-  | Valid ts gs ->
+  | Failed -> Failed
+  | _ ->
     match e with
-    | TOp i e' -> verifier_step_thread e' i vs
+    | Get k v -> vget k v vs
+    | Put k v -> vput k v vs
+    | AddM r k'  -> vaddm r k' vs
+    | EvictM k k' -> vevictm k k' vs
+    | AddB r t j -> vaddb r t j vs
+    | EvictB k t -> vevictb k t vs
+    | EvictBM k k' t -> vevictbm k k' t vs
 
 (* verify a log from a specified initial state *)
-let rec verifier_aux (#p:pos) (l:vlog) (vs:vstate p): Tot (vstate p)
+let rec verifier_thread_aux (#p:pos) (l:vlog) (vs:vtls): Tot vtls
   (decreases (length l)) =
   let n = length l in
   if n = 0 then vs
   else
     let l' = prefix l (n - 1) in
-    let vs' = verifier_aux l' vs in
+    let vs' = verifier_thread_aux l' vs in
     let e' = index l (n - 1) in
-    verifier_step e' vs'
+    verifier_thread_step #p e' vs'
 
 let init_epoch_hash = fun e -> empty_hash_value
 
 let empty_store:vstore = fun (k:key) -> None
 
 (* initialize verifier state *)
-let init_vstate (#p:pos): vstate p = 
-  let gs = GS init_epoch_hash init_epoch_hash in
-  let tls = TLS empty_store (MkTimestamp 0 0) Root in  
-  let tlss = create p tls in
-  let vs:vstate p = Valid tlss gs in
-  let st0 = thread_store 0 vs in
-  let st0_upd = add_to_store st0 Root (init_value Root) Merkle in
-  update_thread_store 0 vs st0_upd
+let init_thread_state (#p:pos) (id:nat{id < p}): vtls = 
+  let vs = Valid id empty_store (MkTimestamp 0 0) Root init_epoch_hash init_epoch_hash in  
+  if id = 0 then
+    let st0 = thread_store vs in
+    let st0_upd = add_to_store st0 Root (init_value Root) MAdd in
+    update_thread_store #p vs st0_upd    
+  else vs
 
-let verifier (#p:pos) (l:vlog): vstate p =
-  verifier_aux l init_vstate
+let verifier_thread (#p:pos) (l:vlog) (id:nat{id < p}): vtls =
+  verifier_thread_aux #p l (init_thread_state id)
 
